LogicGenerator/demo931/impl3.v
@@ -1,0 +1,47 @@
+Require Import Coq.Numbers.BinNums.
+Require Import Coq.PArith.BinPosDef.
+Require Import Logic.lib.PTree.
+Require Import Coq.Sets.Ensembles.
+Require Import Coq.Lists.List.
+Require Import Logic.SeparationLogic.Model.OSAGenerators.
+Require Import Logic.SeparationLogic.Model.SeparationAlgebra.
+Require Import ZArith.
+Require Import QArith.
+Require Import Lqa.
+Import ListNotations.
+
+Definition Q_Join := fun q1 q2 q => 
+  0 <= q1 /\ 0 <= q2 /\ 0 <= q /\ q1 <= 1 /\ q2 <= 1 /\ q <= 1 /\ Qeq q (q1 + q2).
+Definition Q_SA : @SeparationAlgebra Q Q_Join.
+Proof.
+  constructor; intros; unfold join, Q_Join in *;
+  [| exists (mxyz - mx)]; repeat (split; try tauto; lra).
+Qed.
+
+Definition var : Type := nat.
+Definition val : Type := Z.
+Definition addr : Type := nat.
+Definition store : Type := var -> val.
+Definition ASD : Type := Z.
+Definition memval : Type := Q * Z.
+Definition memlock : Type := Q * option Datatypes.unit * ASD.
+Definition heap : Type := addr -> option (memval + memlock).
+
+Definition store_Join := @equiv_Join store.
+Definition memval_Join := @prod_Join Q Z Q_Join equiv_Join.
+Check @option_Join.
+Definition bool_Join := @option_Join Datatypes.unit (@trivial_Join Datatypes.unit).
+Definition QB_Join := @prod_Join Q (option Datatypes.unit) Q_Join bool_Join.
+Definition memlock_Join := @prod_Join _ _ QB_Join (@equiv_Join ASD).
+Check @sum_Join.
+Definition mem_Join := @sum_Join memval memlock memval_Join memlock_Join.
+
+
+Definition heap_Join := @fun_Join addr (option (Q * val)) (@option_Join (Q*val) QV_Join).
+
+
+Module NaiveLang.
+  Definition model : Type := store * heap.
+  Definition join := @prod_Join store 
+
+
